Update append_log output

src/go_lang/examples/append_log.v
@@ -4,6 +4,12 @@ From Perennial.go_lang Require Import prelude.
 (* disk FFI *)
 From Perennial.go_lang Require Import ffi.disk_prelude.
 
+(* Append-only, sequential, crash-safe log.
+
+   The main interesting feature is that the log supports multi-block atomic
+   appends, which are implemented by atomically updating an on-disk header with
+   the number of valid blocks in the log. *)
+
 Module Log.
   Definition S := struct.decl [
     "sz" :: uint64T;
@@ -21,7 +27,7 @@ Definition Log__writeHdr: val :=
   λ: "log",
     let: "hdr" := NewSlice byteT #4096 in
     UInt64Put "hdr" (Log.get "sz" "log");;
-    UInt64Put (SliceSkip "hdr" #8) (Log.get "sz" "log");;
+    UInt64Put (SliceSkip "hdr" #8) (Log.get "diskSz" "log");;
     disk.Write #0 "hdr".
 Theorem Log__writeHdr_t: ⊢ Log__writeHdr : (Log.T -> unitT).
 Proof. typecheck. Qed.
@@ -45,6 +51,19 @@ Definition Init: val :=
 Theorem Init_t: ⊢ Init : (uint64T -> (Log.T * boolT)).
 Proof. typecheck. Qed.
 Hint Resolve Init_t : types.
+
+Definition Open: val :=
+  λ: <>,
+    let: "hdr" := disk.Read #0 in
+    let: "sz" := UInt64Get "hdr" in
+    let: "diskSz" := UInt64Get (SliceSkip "hdr" #8) in
+    struct.mk Log.S [
+      "sz" ::= "sz";
+      "diskSz" ::= "diskSz"
+    ].
+Theorem Open_t: ⊢ Open : (unitT -> Log.T).
+Proof. typecheck. Qed.
+Hint Resolve Open_t : types.
 
 Definition Log__Get: val :=
   λ: "log" "i",
